Renaming + Fix typo

basis/pure/mlsexpScript.sml
@@ -1,5 +1,5 @@
 (*
-  Definition of a simple mlstring-based s-expression, incldues
+  Definition of a simple mlstring-based s-expression, includes
   parsing and pretty printing for these s-expressions.
 *)
 Theory mlsexp
@@ -24,64 +24,64 @@ Datatype:
   token = OPEN | CLOSE | SYMBOL mlstring
 End
 
-Definition read_quoted_aux_def:
-  read_quoted_aux [] acc = NONE ∧
-  read_quoted_aux (#"\""::rest) acc =
+Definition read_string_aux_def:
+  read_string_aux [] acc = NONE ∧
+  read_string_aux (#"\""::rest) acc =
     SOME (implode (REVERSE acc), rest) ∧
-  read_quoted_aux (#"\\"::#"\""::rest) acc =
-    read_quoted_aux rest (#"\""::acc) ∧
-  read_quoted_aux (#"\\"::#"\\"::rest) acc =
-    read_quoted_aux rest (#"\\"::acc) ∧
-  read_quoted_aux (c::cs) acc =
-    read_quoted_aux cs (c::acc)
+  read_string_aux (#"\\"::#"\""::rest) acc =
+    read_string_aux rest (#"\""::acc) ∧
+  read_string_aux (#"\\"::#"\\"::rest) acc =
+    read_string_aux rest (#"\\"::acc) ∧
+  read_string_aux (c::cs) acc =
+    read_string_aux cs (c::acc)
 End
 
 (* Returns the string until a closing quote, and the rest of the input.
    Fails if closing quotes are missing. *)
-Definition read_quoted_def:
-  read_quoted (input: string) : (mlstring # string) option =
-    read_quoted_aux input []
+Definition read_string_def:
+  read_string (input: string) : (mlstring # string) option =
+    read_string_aux input []
 End
 
-Theorem read_quoted_aux_length:
+Theorem read_string_aux_length:
   ∀input acc.
-    read_quoted_aux input acc = SOME (s, rest) ⇒ LENGTH rest ≤ LENGTH input
+    read_string_aux input acc = SOME (s, rest) ⇒ LENGTH rest ≤ LENGTH input
 Proof
-  ho_match_mp_tac read_quoted_aux_ind \\ rw[]
+  ho_match_mp_tac read_string_aux_ind \\ rw[]
   \\ pop_assum mp_tac
-  \\ once_rewrite_tac[read_quoted_aux_def]
+  \\ once_rewrite_tac[read_string_aux_def]
   \\ EVERY_CASE_TAC
   \\ rpt strip_tac \\ res_tac \\ gvs[]
 QED
 
-Theorem read_quoted_length:
-  read_quoted input = SOME (s, rest) ⇒ LENGTH rest ≤ LENGTH input
+Theorem read_string_length:
+  read_string input = SOME (s, rest) ⇒ LENGTH rest ≤ LENGTH input
 Proof
-  rw[read_quoted_def] \\ imp_res_tac read_quoted_aux_length
+  rw[read_string_def] \\ imp_res_tac read_string_aux_length
 QED
 
-Definition read_atom_aux_def:
-  read_atom_aux [] acc =
+Definition read_symbol_aux_def:
+  read_symbol_aux [] acc =
     (implode (REVERSE acc), []) ∧
-  read_atom_aux (c::cs) acc =
+  read_symbol_aux (c::cs) acc =
     if MEM c ") \t\n" then (implode (REVERSE acc), (c::cs))
-    else read_atom_aux cs (c::acc)
+    else read_symbol_aux cs (c::acc)
 End
 
 (* Returns the string until a closing parenthesis or whitespace, and the
    rest of the input. *)
-Definition read_atom_def:
-  read_atom (input: string) : (mlstring # string) =
-    read_atom_aux input []
+Definition read_symbol_def:
+  read_symbol (input: string) : (mlstring # string) =
+    read_symbol_aux input []
 End
 
-Theorem read_atom_aux_length:
+Theorem read_symbol_aux_length:
   ∀input acc.
-    read_atom_aux input acc = (s, rest) ⇒ LENGTH rest ≤ LENGTH input
+    read_symbol_aux input acc = (s, rest) ⇒ LENGTH rest ≤ LENGTH input
 Proof
   Induct
-  \\ simp[read_atom_aux_def]
-  \\ rw[read_atom_aux_def] \\ res_tac \\ gvs[]
+  \\ simp[read_symbol_aux_def]
+  \\ rw[read_symbol_aux_def] \\ res_tac \\ gvs[]
 QED
 
 (* Where possible, we return our progress, and the rest of the input.
@@ -101,23 +101,23 @@ Definition lex_aux_def:
        else if depth = 1 then INR (CLOSE::acc, cs)
        else lex_aux (depth - 1) cs (CLOSE::acc))
     else if c = #"\"" then
-      case read_quoted cs of
+      case read_string cs of
       | NONE => INL (acc, c::cs)
       | SOME (s, rest) =>
           if depth = 0 then INR ([SYMBOL s], rest)
           else lex_aux depth rest ((SYMBOL s)::acc)
     else
-      case read_atom (c::cs) of
+      case read_symbol (c::cs) of
       | (s, rest) =>
           if depth = 0 then INR ([SYMBOL s], rest)
           else lex_aux depth rest ((SYMBOL s)::acc)
 Termination
   wf_rel_tac ‘measure $ (λ(_, input, _). LENGTH input)’ \\ rw[]
-  \\ imp_res_tac read_quoted_length \\ fs[]
-  \\ fs[read_atom_def]
-  \\ fs[Once read_atom_aux_def]
+  \\ imp_res_tac read_string_length \\ fs[]
+  \\ fs[read_symbol_def]
+  \\ fs[Once read_symbol_aux_def]
   \\ gvs [AllCaseEqs()]
-  \\ imp_res_tac read_atom_aux_length \\ fs[]
+  \\ imp_res_tac read_symbol_aux_length \\ fs[]
 End
 
 (* Tokenizes (at most) one S-expression, and returns the rest of the input. *)
